src/Find_tree_stack.thy
@@ -15,6 +15,7 @@ done
 definition tree_to_fts :: "key => Tree => fts_state_t" where
 "tree_to_fts k t = (Focus(k,None,t,None),Nil)"
 
+
 (*
 definition focus_to_map :: "fts_focus_t \<Rightarrow> (key \<Rightarrow> value_t option)" where
 "focus_to_map f = (
@@ -27,10 +28,11 @@ definition focus_to_map :: "fts_focus_t \<Rightarrow> (key \<Rightarrow> value_t
 (* tr: link between focus and context?*)
 (*begin wf fts focus definition*)
 
+(*
 FIXME we also need that, not only is the focus bounded, but any key in the bound must be in the leaves of this tree
 
 its not just that lu is a bound, it is that the subtree is the unique subtree which contains entries from this bound
-
+*)
 
 
 definition wellformed_fts_focus :: "key \<Rightarrow> ms_t \<Rightarrow> fts_focus_t => bool" where
@@ -45,17 +47,17 @@ definition wellformed_fts_focus :: "key \<Rightarrow> ms_t \<Rightarrow> fts_foc
 (*begin wf fts1 definition*)
 (* tr: interaction between focus and context *)
 definition wellformed_fts_1 :: "fts_state_t => bool" where
-"wellformed_fts_1 fts == (
+"wellformed_fts_1 fts = (
   let (f,ts) = fts in
   case ts of
   Nil => True
   | cn#xs => (    
     let (k,l,t,u) = dest_fts_focus f in
-    let (l,ks,rs,i,u) = dest_cnode_t cn in
+    let (_,_,rs,i,_) = dest_cnode cn in
     let b0 = (t = rs!i) in
     let b2 = (cnode_to_bound cn = (l,u)) in  (* ensure bounds are linked *)
-    b0&b2))
-"
+    b0&b2)
+)"
 (*end wf fts1 definition*)
 
 (*begin wf fts definition*)
@@ -63,7 +65,7 @@ definition wellformed_fts :: "key \<Rightarrow> fts_state_t => bool" where
 "wellformed_fts k0 fts = (
   let (f,ts) = fts in
   let ms = ts_to_ms ts in
-  wellformed_context k0 ts
+  wellformed_ts k0 ts
   & wellformed_fts_focus k0 ms f
   & wellformed_fts_1 fts)"
 (*end wf fts definition*)
@@ -102,23 +104,45 @@ definition fts_reass :: "fts_state_t \<Rightarrow> Tree" where
 (* lemmas ------------------------------------------- *)
 
 (*begin find invariant*)
-definition invariant_wf_fts :: "key \<Rightarrow> bool" where
-"invariant_wf_fts k0 = (! fts fts'.
+definition invariant_wf_fts :: "bool" where
+"invariant_wf_fts = (! k0 fts fts'.
   (step_fts fts = Some (fts')) &
   wellformed_fts k0 fts \<longrightarrow> wellformed_fts k0 fts')
 "
 (*end find invariant*)
 
+(* prefer lem2; k0 is located in the focus; proof by induction on ts; perhaps better to do this for the step case explicitly?*)
+definition lem1 :: "bool" where
+"lem1 = (
+  ! k0 f ts.
+  let (k,l,t,u) = dest_fts_focus f in
+  let (ks,rs) = ts_to_t0 ts |> dest_Some in
+  (ts \<noteq> []) &
+  wellformed_fts k0 (f,ts) & 
+  k0 : tree_to_map (Node(ks,rs)) |> dom \<longrightarrow>
+  k0 : tree_to_map t |> dom 
+)"
+
+definition lem2 :: "bool" where
+"lem2 = (! k0 f ts f' ts'.
+  let (_,_,t,_) = dest_fts_focus f in
+  let (_,_,t',_) = dest_fts_focus f' in
+  wellformed_fts k0 (f,ts) &
+  k0 : (t|>tree_to_map|>dom) &
+  (step_fts (f,ts) = Some(f',ts')) \<longrightarrow>
+  k0 : (t'|>tree_to_map|>dom)
+)"
+
+
 definition lemma_fts_reass :: "bool" where
 "lemma_fts_reass = (! k0 f ts.
   wellformed_fts k0 (f,ts) \<longrightarrow> (
-  let (k,l,t,u) = dest_fts_focus f in
+  let (k,_,t,_) = dest_fts_focus f in
   ? xs zs. 
-    (fts_reass (f,ts) |> tree_to_leaves = xs@(tree_to_leaves t)@zs) & 
-    (let ks = xs |> leaves_to_map |> dom in check_keys None ks l) &
-    (check_keys l (t|>tree_to_leaves|>leaves_to_map|>dom) u) &
-    (let ks = zs |> leaves_to_map |> dom in check_keys u ks None)
-))"  
+    let t' = fts_reass (f,ts) in 
+    (t' |> tree_to_leaves = xs@(tree_to_leaves t)@zs) & 
+    (k0 : tree_to_map t' |> dom \<longrightarrow> k0 : tree_to_map t |> dom))
+)"  
 
 
 
